src/tls/IdNonce.fst
@@ -1,0 +1,53 @@
+(* This module maintains a injective monotonic map from nonces to ids *)
+module IdNonce
+open TLSConstants
+open Platform.Bytes
+open Platform.Error
+open TLSInfo
+
+module N=Nonce
+module MM = MonotoneMap
+module MR = FStar.Monotonic.RRef
+module HH = FStar.HyperHeap
+
+val nonce_of_id : i:id -> Tot N.random
+let nonce_of_id i = fst (Platform.Bytes.split i.csrConn 32)
+
+//The goal of the rest of the module is to provide id_of_nonce
+//and to prove that the two are mutual inverses
+type n_id (n:random) = i:id{nonce_of_id i = n}
+
+//nonce_id_table:
+//  A monotone, injective partial map in the tls_tables_region, from random to rid
+let nonce_id_table : MM.t tls_tables_region random n_id (fun x -> True) =
+  MM.alloc #tls_tables_region #random #n_id #(fun x -> True)
+
+let id_of_nonce (n:random) (i:n_id n) = MR.witnessed (MM.contains nonce_id_table n i)
+
+val insert: n:random -> i:n_id n -> ST unit
+  (requires (fun h -> MM.sel (MR.m_sel h nonce_id_table) n = None))
+  (ensures (fun h0 _ h1 -> 
+      HH.modifies (Set.singleton tls_tables_region) h0 h1 /\
+      HH.modifies_rref tls_tables_region !{HH.as_ref (MR.as_rref nonce_id_table)} h0 h1 /\
+      id_of_nonce n i))
+let insert n i = 
+  MR.m_recall nonce_id_table;
+  MM.extend nonce_id_table n i 
+
+val lookup: n:random -> ST (option (n_id n))
+  (requires (fun h -> True))
+  (ensures (fun h0 idopt h1 -> 
+    h0=h1 /\
+    idopt = MM.sel (MR.m_sel h0 nonce_id_table) n /\
+    (match idopt with 
+     | None -> True
+     | Some i -> id_of_nonce n i)))
+let lookup n = MM.lookup nonce_id_table n     
+
+val injectivity : n:random -> m:random -> i:n_id n -> j:n_id m ->  ST unit
+  (requires (fun h -> i<>j /\ id_of_nonce n i /\ id_of_nonce m j))
+  (ensures (fun h0 _ h1 -> n<>m))
+let injectivity n m i j =
+  MR.testify (MM.contains nonce_id_table n i);
+  MR.testify (MM.contains nonce_id_table m j)
+  
